TyTests/CtorFnTest/UseModule.lean
@@ -1,0 +1,6 @@
+import TyTests.CtorFnTest.Module
+open LeanScript CtorFnModuleTest
+example : Term.run (Sg := ⟨[], rfl⟩) PUnit.unit pt = (1, 2, ()) := rfl
+def some4 : Term ⟨[], rfl⟩ [] (#leanscript_layout `Option `some natT) :=
+  #leanscript_ctor `Option `some natT (.nat_mk 4)
+#print some4
